\documentclass[12pt]{beamer}
\usetheme{Warsaw}
\usepackage[utf8]{inputenc}
\usepackage{amsmath}
\usepackage{amsfonts}
\usepackage{amssymb}
\usepackage{graphicx}
\usepackage[font=Times,timeinterval=1,timeduration=2.0,timedeath=0,fillcolorwarningsecond=white!60!yellow,timewarningfirst=50,timewarningsecond=80,resetatpages=2]{tdclock}
\usepackage{tabularx}
\usepackage{array}
\usepackage{multicol}
\usepackage{longtable}
\usepackage{xcolor}
\usepackage{textcomp, gensymb}
\usepackage{pgfplots}
\usepackage[makeroom]{cancel}

\graphicspath{ {./references/} }
\pgfplotsset{
	soldot/.style={color=black,only marks,mark=*},
	holdot/.style={color=black,fill=white,only marks,mark=*},
	compat=1.12
}
\newcolumntype{Y}{>{\centering\arraybackslash}X}
\makeatletter
\def\@listii{\leftmargin\leftmarginii
			  \topsep    2ex
			  \parsep    0\p@   \@plus\p@
			  \itemsep   \parsep}
\makeatother
\newcommand\at[2]{\left.#1\right|_{#2}}

\begin{document}
\begin{frame}
	\frametitle{Bellwork 12/8}
	\initclock

	\vfill
	\LARGE
	\[f(x)=\ln(x)+2\]
	\vfill
	\begin{center}
		Find $(f^{-1})^{'}(2)$.
	\end{center}
	\vfill
	\vfill
	\vfill
	\vfill
	\vfill
	\vfill

	\small
	\crono
	\resetcrono{\beamerbutton{reset}}
\end{frame}
\begin{frame}
	\frametitle{Bellwork 12/8 - Solution 1}

	\Large
	\[x=\ln[f^{-1}(x)]+2\]
	\[\implies f^{-1}(x)=e^{x-2}\]
	\[\implies (f^{-1})^{'}(x)=e^{x-2}\]
	\vfill
	\[\therefore \boxed{(f^{-1})^{'}(2)=1}\]
\end{frame}
\begin{frame}
	\frametitle{Bellwork 12/8 - Solution 2}

	\Large
	\[f'(x)=\frac{1}{x}\text{; }f^{-1}(x)=e^{x-2}\]
	\vfill
	\[(f^{-1})^{'}(x)=\frac{1}{f'[f^{-1}(x)]}\]
	\[\implies (f^{-1})^{'}(2)=\frac{1}{f'[f^{-1}(2)]}=\frac{1}{f'(1)}=\boxed{1}\]
\end{frame}
\begin{frame}
	\frametitle{Exercise 1}

	\Large
	Find the general antiderivative of $f$:
	\[f(x)=\frac{1}{5}-\frac{2}{x}\]
\end{frame}
\begin{frame}
	\frametitle{Exercise 2}

	\Large
	Find the general antiderivative of $g$:
	\[g(t)=\frac{3t^4-t^3+4}{t^4}\]
\end{frame}
\begin{frame}
	\frametitle{Exercise 3}

	\Large
	Find the general antiderivative of $h$:
	\[h(s)=\frac{1+s^2+s}{\sqrt{s}}\]
\end{frame}
\end{document}