\documentclass[12pt]{beamer}
\usetheme{Warsaw}
\usepackage[utf8]{inputenc}
\usepackage{amsmath}
\usepackage{amsfonts}
\usepackage{amssymb}
\usepackage{graphicx}
\usepackage[font=Times,timeinterval=1,timeduration=2.0,timedeath=0,fillcolorwarningsecond=white!60!yellow,timewarningfirst=50,timewarningsecond=80,resetatpages=2]{tdclock}
\usepackage{tabularx}
\usepackage{array}
\usepackage{multicol}
\usepackage{longtable}
\usepackage{xcolor}
\usepackage{textcomp, gensymb}
\usepackage{pgfplots}
\usepackage[makeroom]{cancel}

\graphicspath{ {./references/} }
\pgfplotsset{
	soldot/.style={color=black,only marks,mark=*},
	holdot/.style={color=black,fill=white,only marks,mark=*},
	compat=1.12
}
\newcolumntype{Y}{>{\centering\arraybackslash}X}
\makeatletter
\def\@listii{\leftmargin\leftmarginii
			  \topsep    2ex
			  \parsep    0\p@   \@plus\p@
			  \itemsep   \parsep}
\makeatother
\newcommand\at[2]{\left.#1\right|_{#2}}

\begin{document}
\begin{frame}
	\frametitle{Bellwork 10/25}
	\initclock

	\vfill
	\vfill
	\vfill
	\vfill
	\Large
	Find $\frac{\mathrm{d}y}{\mathrm{d}x}$ of the implicitly defined curve:
	\[x^3+xy^2+y=x^2y\]
	\vfill
	\vfill
	\vfill
	\vfill
	\vfill
	\vfill
	\vfill

	\small
	\crono
	\resetcrono{\beamerbutton{reset}}
\end{frame}
\begin{frame}
	\frametitle{Bellwork 10/25 - Solution}

	\large
	\[3x^2+y^2+2xy\left(\frac{\mathrm{d}y}{\mathrm{d}x}\right)+\frac{\mathrm{d}y}{\mathrm{d}x}=2xy+x^2\left(\frac{\mathrm{d}y}{\mathrm{d}x}\right)\]
	\[(2xy+1-x^2)\left(\frac{\mathrm{d}y}{\mathrm{d}x}\right)=2xy-3x^2-y^2\]
	\[\boxed{\frac{\mathrm{d}y}{\mathrm{d}x}=\frac{2xy-3x^2-y^2}{2xy+1-x^2}}\]
\end{frame}
\begin{frame}
	\frametitle{Exercise 1}

	\large
	Find the equations of the lines tangent to the ellipse below, at $x=-2$: \[\frac{x^{2}}{8}+\frac{y^{2}}{4}=1\]
\end{frame}
\begin{frame}
	\frametitle{Exercise 1 - Solution, Part 1}

	Find $\frac{\mathrm{d}y}{\mathrm{d}x}$:
	\[\frac{x}{4}+\frac{y}{2}\left(\frac{\mathrm{d}y}{\mathrm{d}x}\right)=0\]
	\[\frac{\mathrm{d}y}{\mathrm{d}x}=-\frac{x}{2y}\]
	Find the $y_0$ values (when $x=-2$):
	\[y_0=\pm\sqrt{4\left[1-\frac{(-2)^2}{8}\right]}=\pm\sqrt{2}\]
\end{frame}
\begin{frame}
	\frametitle{Exercise 1 - Solution, Part 2}

	\[\text{Point-Slope Form: }y\pm\sqrt{2}=\at{\frac{\mathrm{d}y}{\mathrm{d}x}}{-2}(x+2)\]
	\[\implies \boxed{y=\frac{1}{\sqrt{2}}(x+2)+\sqrt{2}}\text{; }\boxed{y=-\frac{1}{\sqrt{2}}(x+2)-\sqrt{2}}\]
\end{frame}
\begin{frame}
	\frametitle{Exercise 2}

	\large
	Find the equation of the line tangent to the hyperbola below, at $(2, 2)$: \[\frac{y^{2}}{2}-\frac{x^{2}}{4}=1\]
\end{frame}
\begin{frame}
	\frametitle{Exercise 2 - Solution}

	Find $\frac{\mathrm{d}y}{\mathrm{d}x}$:
	\[y\left(\frac{\mathrm{d}y}{\mathrm{d}x}\right)-\frac{x}{2}=0\]
	\[\frac{\mathrm{d}y}{\mathrm{d}x}=\frac{x}{2y}\]
	\vfill
	\hrule
	\vfill
	\[\text{Point-Slope Form: }y-2=\at{\frac{\mathrm{d}y}{\mathrm{d}x}}{2}(x-2)\]
	\[\implies \boxed{y=\frac{1}{2}(x-2)+2}\]
\end{frame}
\end{document}