\documentclass[12pt]{beamer}
\usetheme{Warsaw}
\usepackage[utf8]{inputenc}
\usepackage{amsmath}
\usepackage{amsfonts}
\usepackage{amssymb}
\usepackage{graphicx}
\usepackage[font=Times,timeinterval=1,timeduration=2.0,timedeath=0,fillcolorwarningsecond=white!60!yellow,timewarningfirst=50,timewarningsecond=80,resetatpages=2]{tdclock}
\usepackage{tabularx}
\usepackage{array}
\usepackage{multicol}
\usepackage{longtable}
\usepackage{xcolor}
\usepackage{textcomp, gensymb}
\usepackage{pgfplots}
\usepackage[makeroom]{cancel}

\graphicspath{ {./references/} }
\pgfplotsset{
	soldot/.style={color=black,only marks,mark=*},
	holdot/.style={color=black,fill=white,only marks,mark=*},
	compat=1.12
}
\newcolumntype{Y}{>{\centering\arraybackslash}X}
\makeatletter
\def\@listii{\leftmargin\leftmarginii
			  \topsep    2ex
			  \parsep    0\p@   \@plus\p@
			  \itemsep   \parsep}
\makeatother
\newcommand\at[2]{\left.#1\right|_{#2}}

\begin{document}
\begin{frame}
	\frametitle{Bellwork 10/30}
	\initclock

	\vfill
	\vfill
	\vfill
	\vfill
	\Large
	\[f(x)=\ln\left(x^{2}+1\right)\]
	\vfill
	\large
	\begin{center}
		Find the equation of the line tangent to $f$ at $x=-1$.
	\end{center}
	\vfill
	\vfill
	\vfill
	\vfill
	\vfill
	\vfill
	\vfill

	\small
	\crono
	\resetcrono{\beamerbutton{reset}}
\end{frame}
\begin{frame}
	\frametitle{Bellwork 10/30 - Solution}

	\vfill
	\vfill
	\vfill
	\Large
	\[f'(x)=\frac{2x}{x^2+1}\]
	\vfill
	\large
	\[\text{Point-Slope Form: }y-f(-1)=f'(-1)(x+1)\]
	\[\implies \boxed{y=-x-1+\ln(2)}\]
	\vfill
	\vfill
	\vfill
\end{frame}
\begin{frame}
	\frametitle{Exercise 1}

	\LARGE
	Find $\frac{\mathrm{d}y}{\mathrm{d}x}$:
	\[y=\frac{(x^2-1)^x}{\sqrt{x+1}}\]
\end{frame}
\begin{frame}
	\frametitle{Exercise 1 - Solution, Part 1}

	\large
	Take the natural logarithm of both sides:
	\[\ln(y)=\ln\left[\frac{(x^2-1)^x}{\sqrt{x+1}}\right]\]
	\[\ln(y)=x\ln(x^2-1)-\frac{1}{2}\ln(x+1)\]
	Implicitly differentiate:
	\[\frac{1}{y}\left(\frac{\mathrm{d}y}{\mathrm{d}x}\right)=\ln(x^2-1)+\frac{2x^2}{x^2-1}-\frac{1}{2x+2}\]
\end{frame}
\begin{frame}
	\frametitle{Exercise 1 - Solution, Part 2}

	\large
	Solve for $\frac{\mathrm{d}y}{\mathrm{d}x}$ and substitute for $y$:
	\[\boxed{\frac{\mathrm{d}y}{\mathrm{d}x}=\left[\frac{(x^2-1)^x}{\sqrt{x+1}}\right]\left[\ln(x^2-1)+\frac{2x^2}{x^2-1}-\frac{1}{2x+2}\right]}\]
\end{frame}
\begin{frame}
	\frametitle{Exercise 2}

	\LARGE
	Find $\frac{\mathrm{d}u}{\mathrm{d}v}$:
	\[u=\frac{v^{\ln(v)}}{\ln(v)}\]
\end{frame}
\begin{frame}
	\frametitle{Exercise 2 - Solution}

	\Large
	\[\ln(u)=\ln(v)\ln(v)-\ln[\ln(v)]\]
	\[\frac{1}{u}\left(\frac{\mathrm{d}u}{\mathrm{d}v}\right)=\frac{2\ln(v)}{v}-\frac{1}{v\ln(v)}\]
	\[\boxed{\frac{\mathrm{d}u}{\mathrm{d}v}=\left[\frac{v^{\ln(v)}}{\ln(v)}\right]\left[\frac{2\ln(v)}{v}-\frac{1}{v\ln(v)}\right]}\]
\end{frame}
\end{document}